extract "Rust" library functions to C relying on Karamel monomorphization

lib/pulse/lib/Pulse.Lib.Vec.fst
@@ -28,9 +28,9 @@ let is_full_vec v = A.is_full_array v
 let pts_to v #p s = A.pts_to v #p s
 let pts_to_len v = A.pts_to_len v
 let alloc x n = A.alloc x n
-let op_Array_Access v i = A.op_Array_Access v i
-let op_Array_Assignment v i x = A.op_Array_Assignment v i x
-let free v = A.free v
+let op_Array_Access #a v i #p #s = A.opArrayAccess0 #a #p #s v i
+let op_Array_Assignment #a v i x #s = A.opArrayAssignment0 v i x
+let free #a v #s = A.free0 #a #s v
 let share v = A.share v
 let gather v = A.gather v
 
